main preservation theorem done

theories/host.v
@@ -51,9 +51,9 @@ Record host := {
       store_typing st ->
       store_typing st' (** [host_application] preserves store typing. **) ;
     host_application_respect : forall s t1s t2s st h vs s' st' r,
-      all2 types_agree t1s vs ->
+      values_typing st vs = Some t1s ->
       host_application s st (Tf t1s t2s) h vs s' (Some (st', r)) ->
-      result_types_agree t2s r (** [host_application] respects types. **)
+      result_types_agree st' t2s r (** [host_application] respects types. **)
   }.
 
 End Predicate.
